AssemblyLanguage.thy
@@ -1,0 +1,100 @@
+theory AssemblyLanguage
+imports MachineLanguage FiniteMap Iterate
+begin
+
+typedecl symbol
+
+datatype assembly =
+  AAssm int
+| SAssm symbol
+| CAssm "register set" computation "comparison set"
+
+type_synonym program = "symbol \<leadsto> assembly list"
+
+type_synonym assembly_state = "memory \<times> int \<times> int \<times> symbol \<times> assembly list" (* M, A, D, S, PC *)
+
+fun eval_assembly :: "program \<Rightarrow> assembly_state \<Rightarrow> assembly_state option" where
+  "eval_assembly \<Pi> (\<sigma>, a, d, s, []) = None"
+| "eval_assembly \<Pi> (\<sigma>, a, d, s, AAssm x # \<pi>) = Some (\<sigma>, x, d, s, \<pi>)"
+| "eval_assembly \<Pi> (\<sigma>, a, d, s, SAssm x # \<pi>) = Some (\<sigma>, a, d, x, \<pi>)"
+| "eval_assembly \<Pi> (\<sigma>, a, d, s, CAssm dst cmp jmp # \<pi>) = (
+    let n = compute cmp (\<sigma> (nat a)) a d
+    in let \<sigma>' = if M \<in> dst then \<sigma>(nat a := n) else \<sigma>
+    in let a' = if A \<in> dst then n else a
+    in let d' = if D \<in> dst then n else d
+    in if should_jump n jmp
+       then case lookup \<Pi> s of 
+           Some \<pi>' \<Rightarrow> Some (\<sigma>', a', d', s, \<pi>')
+         | None \<Rightarrow> None
+       else Some (\<sigma>', a', d', s, \<pi>))"
+
+(* conversion *)
+
+fun block_size :: "assembly list \<Rightarrow> nat" where
+  "block_size [] = 0"
+| "block_size (AAssm x # as) = Suc (block_size as)"
+| "block_size (SAssm x # as) = block_size as"
+| "block_size (CAssm dst cmp jmp # as) = Suc (block_size as)"
+
+fun build_symbol_table :: "program \<Rightarrow> symbol \<rightharpoonup> nat" where
+  "build_symbol_table [] s = None"
+| "build_symbol_table ((s', \<pi>) # \<Pi>) s = (
+    if s' = s 
+    then Some 0 
+    else map_option (op + (block_size \<pi>)) (build_symbol_table \<Pi> s))"
+
+primrec instruction_conv :: "(symbol \<rightharpoonup> nat) \<Rightarrow> assembly \<Rightarrow> instruction" where
+  "instruction_conv \<rho> (AAssm x) = AInstr x"
+| "instruction_conv \<rho> (SAssm x) = AInstr (int (the (\<rho> x)))"
+| "instruction_conv \<rho> (CAssm dst cmp jmp) = CInstr dst cmp jmp"
+
+fun program_convert' :: "(symbol \<rightharpoonup> nat) \<Rightarrow> program \<Rightarrow> instruction list" where
+  "program_convert' \<rho> [] = []"
+| "program_convert' \<rho> ((s, \<pi>) # \<Pi>) = map (instruction_conv \<rho>) \<pi> @ program_convert' \<rho> \<Pi>"
+
+definition program_convert :: "program \<Rightarrow> instruction list" where
+  "program_convert \<Pi> = program_convert' (build_symbol_table \<Pi>) \<Pi>"
+
+fun state_convert :: "program \<Rightarrow> assembly_state \<Rightarrow> machine_state" where
+  "state_convert \<Pi> (\<sigma>, a, d, s, \<pi>) = (\<sigma>, a, d, undefined)"
+
+(* conversion correctness *)
+
+lemma [simp]: "eval_assembly \<Pi> \<sigma> = Some \<sigma>\<^sub>1 \<Longrightarrow> 
+    iterate (eval (program_convert \<Pi>)) (state_convert \<Pi> \<sigma>) (state_convert \<Pi> \<sigma>\<^sub>1)"
+  proof (induction \<Pi> \<sigma> rule: eval_assembly.induct)
+  case (1 \<Pi> \<sigma> a d s)
+    thus ?case by simp
+  next case (2 \<Pi> \<sigma> a d s x \<pi>)
+    hence "eval_assembly \<Pi> (\<sigma>, a, d, s, AAssm x # \<pi>) = Some \<sigma>\<^sub>1" by simp
+
+
+
+    have "iterate (eval (program_convert \<Pi>)) (state_convert \<Pi> (\<sigma>, a, d, s, AAssm x # \<pi>)) (state_convert \<Pi> \<sigma>\<^sub>1)" by simp
+    thus ?case by simp
+  next case (3 \<Pi> \<sigma> a d s x \<pi>)
+    hence "eval_assembly \<Pi> (\<sigma>, a, d, s, SAssm x # \<pi>) = Some \<sigma>\<^sub>1" by simp
+
+
+
+    have "iterate (eval (program_convert \<Pi>)) (state_convert \<Pi> (\<sigma>, a, d, s, SAssm x # \<pi>)) (state_convert \<Pi> \<sigma>\<^sub>1)" by simp
+    thus ?case by simp
+  next case (4 \<Pi> \<sigma> a d s dst cmp jmp \<pi>)
+    hence "eval_assembly \<Pi> (\<sigma>, a, d, s, CAssm dst cmp jmp # \<pi>) = Some \<sigma>\<^sub>1" by simp
+
+
+
+    have "iterate (eval (program_convert \<Pi>)) (state_convert \<Pi> (\<sigma>, a, d, s, CAssm dst cmp jmp # \<pi>)) (state_convert \<Pi> \<sigma>\<^sub>1)" by simp
+    thus ?case by simp
+  qed
+
+theorem [simp]: "iterate (eval_assembly \<Pi>) \<sigma> \<sigma>\<^sub>1 \<Longrightarrow> 
+    iterate (eval (program_convert \<Pi>)) (state_convert \<Pi> \<sigma>) (state_convert \<Pi> \<sigma>\<^sub>1)"
+  proof (induction "eval_assembly \<Pi>" \<sigma> \<sigma>\<^sub>1 rule: iterate.induct) 
+  case iter_refl
+    thus ?case by simp
+  next case iter_step
+    thus ?case by fastforce
+  qed
+
+end
