FiniteMap.thy
@@ -1,0 +1,11 @@
+theory FiniteMap
+imports Main
+begin
+
+type_synonym ('a, 'b) finite_map = "('a \<times> 'b) list" (infixr "\<leadsto>" 50)
+
+fun lookup :: "'a \<leadsto> 'b \<Rightarrow> 'a \<rightharpoonup> 'b" where
+  "lookup [] k = None"
+| "lookup ((a, b) # ab) k = (if a = k then Some b else lookup ab k)"
+
+end
