Iterate.thy
@@ -1,0 +1,28 @@
+theory Iterate
+imports Main
+begin
+
+inductive iterate :: "('a \<rightharpoonup> 'a) \<Rightarrow> 'a \<Rightarrow> 'a \<Rightarrow> bool" where 
+  iter_refl [simp]: "iterate f x x"
+| iter_step [simp]: "iterate f x y \<Longrightarrow> f y = Some z \<Longrightarrow> iterate f x z"
+
+lemma [elim]: "f x = Some y \<Longrightarrow> iterate f x y"
+  proof -
+    assume "f x = Some y"
+    moreover have "iterate f x x" by simp
+    ultimately show "iterate f x y" by (metis iter_step)
+  qed
+
+lemma [elim]: "iterate f y z \<Longrightarrow> f x = Some y \<Longrightarrow> iterate f x z"
+  by (induction f y z rule: iterate.induct) auto
+
+lemma [elim]: "iterate f x y \<Longrightarrow> iterate f y z \<Longrightarrow> iterate f x z"
+  proof (induction f x y rule: iterate.induct)
+  case iter_refl
+    thus ?case by simp
+  next case (iter_step f x y w)
+    hence "iterate f y z" by auto
+    with iter_step show ?case by simp
+  qed
+
+end
